iris/UInitConsK.v
@@ -227,6 +227,7 @@ Section UInitConsK.
        of_Fex   := pfam_triv (fun _ _ _ _ => True%I);
        of_Fo    := pfam_triv (fun _ _ _ => True%I);
        of_Ft    := pfam_triv (fun _ _ _ => True%I);
+       of_om    := OffParked;
        wf_Q     := fun _ => True%I;
        nf_P     := P;
        nf_Pmiss := fun _ _ => True%I;
